epic ptr system refactoring

src/Pointer.v
@@ -1,118 +1,222 @@
 From RecordUpdate Require Import RecordSet.
 Require Memory.
 
-Import Bool Core ZMod Common MemoryBase Memory RecordSetNotations ZMod PMap_ext BinInt.
+Import Bool Core ZMod Common MemoryBase Memory RecordSetNotations PMap_ext BinInt.
 
 Section Definitions.
-
   Open Scope ZMod_scope.
-  (** # Fat Pointers
+  (** This file describes three concepts related to [data_page]s: spans, heap pointers, fat pointers.
+
+# Span
+
+A **span** is a range of addresses on some [data_page] from [%start] inclusive to [%start + length] exclusive.
+
+*)
+  Record span :=
+    mk_span {
+        s_start: mem_address;
+        s_length: mem_address;
+      }.
+  Inductive span_limit : span -> mem_address -> Prop :=
+    | sl_apply: forall s l limit,
+        s + l = (limit, false) ->
+        span_limit (mk_span s l) limit.
+  
+  (**
 
 A **fat pointer** defines an address inside a slice of a data memory page.
 
-The slice begins on page with ID=[fp_page] starting at [fp_start] (inclusive) and ending at
-[fp_start]+[fp_length] (exclusive).
+The slice begins on page with ID=[%fp_page] starting at [%fp_start] (inclusive) and ending at
+[%fp_start]+[%fp_length] (exclusive).
+These four components are enough to unambiguously identify a slice of a data memory page.
+
+Note, that fat pointers are not always marked with a pointer tag! See the details below.
 *)
+
+  Record heap_ptr :=
+    mk_hptr
+      {
+        hp_addr: mem_address;
+        hp_limit: mem_address;
+      }.
+
+  Inductive hp_resolves_to : heap_ptr -> mem_address -> Prop :=
+    | tpr_apply: forall addr limit,
+      ( addr < limit ) = true ->
+      hp_resolves_to (mk_hptr addr limit) addr.
+
+  Record free_ptr :=
+    mk_ptr {
+        p_span :> span;
+        p_offset: mem_address;
+      }.
+  Definition fresh_ptr (s:span) : free_ptr :=
+    mk_ptr s zero32.
+
+  Definition validate_in_bounds (p:free_ptr) : bool :=  p.(p_offset) < p.(s_length) .
+
+  Inductive ptr_resolves_to : free_ptr -> mem_address -> Prop :=
+    | upr_apply: forall addr start ofs length,
+      (addr, false) = start + ofs ->
+      ( ofs < length ) = true ->
+      ptr_resolves_to (mk_ptr (mk_span start length) ofs) addr.
+
   Record fat_ptr :=
     mk_fat_ptr {
         fp_page: option page_id;
-        fp_start: mem_address;
-        fp_length: mem_address;
-        fp_offset: mem_address;
+        fp_ptr :> free_ptr;
       }.
 
-  #[export] Instance etaFatPointer: Settable _
-    := settable! mk_fat_ptr < fp_page; fp_start; fp_length; fp_offset>.
-(** The absolute address encoded by a fat pointer is [fp_start + fp_offset].
-In order to dereference it, the address should be in bounds, therefore,
+  Definition heap_ptr_span (hp:heap_ptr) : span := mk_span zero32 hp.(hp_limit).
+  Definition heap_ptr_to_free (hp:heap_ptr) : free_ptr := mk_ptr (heap_ptr_span hp) hp.(hp_addr).
+
+
+  Definition fatten (hp: free_ptr) (pid: page_id) : fat_ptr :=
+    mk_fat_ptr (Some pid) hp.
+
+  Inductive fp_lift (P: free_ptr -> free_ptr -> Prop) : fat_ptr -> fat_ptr -> Prop :=
+    |fpl_apply: forall i p1 p2, P p1 p2 ->
+                fp_lift P (mk_fat_ptr i p1) (mk_fat_ptr i p2).
+
+  #[export] Instance etaSpan : Settable _ := settable! mk_span < s_start; s_length >.
+  #[export] Instance etaFreePointer: Settable _ := settable! mk_ptr < p_span; p_offset >.
+  #[export] Instance etaFatPointer: Settable _ := settable! mk_fat_ptr < fp_page; fp_ptr >.
+
+  (** ## Usage
+
+- Fat pointers are used to pass read-only spans of memory between contracts, either through [%OpFarCall]/[%OpMimicCall]/[%OpDelegateCall] or through [%OpFarRet]/[%OpFarRevert].
+
+- Fat pointers are used by instructions [%OpLoad], [%OpLoadInc], [%OpStore], [%OpStoreInc], [%OpLoadPointer], [%OpLoadPointerInc].
+
+
+
+Pointers may be created only by far calls ([%OpFarCall], [%OpMimicCall], [%OpDelegateCall]) or far returns ([%OpFarRet], [%OpFarRevert]).
+
+- They are used to forward data spans between contracts.
+
+- Pointers are created as **fresh**: their [%fp_start = 0] and [%fp_offset = 0].
+- Instructions [%OpPtrPack], [%OpPtrShrink], [%OpPtrAdd] and [%OpPtrSub] are used to manipulate them; 
+
+## Validation
+
+- Valid fat pointers to heap variants always have [%fp_start = 0], therefore [%fp_offset] is an absolute address in the heap variant.
+
+
+The absolute address encoded by a fat pointer is [%fp_start + fp_offset].
+In order to dereference it, the address should be in bounds; this is formalized
+by a function [%validate_in_bounds].
 **)
-  Definition validate_in_bounds (p:fat_ptr) : bool := (lt_unsigned _ p.(fp_offset) p.(fp_length) ).
-
-  (** Note: Valid heap/auxheap fat pointers always have [fp_start = 0], therefore
-[fp_offset] is an absolute address in (aux_)heap.
 
 
-## Usage
-
-- Fat pointers are used to pass read-only slices of memory between contracts, either through [OpFarCall]/[OpMimicCall]/[OpDelegateCall] or through `ret`/`revert`.
-- Fat pointers are used by instructions [OpLoad], [OpLoadInc], [OpStore], [OpStoreInc], [OpLoadPointer], [OpLoadPointerInc].
-Additionally, they are used to forward data slices between external frames.
-Pointers are created and managed by [OpPtrAdd], [OpPtrSub], [OpPtrPack] and [OpPtrShrink] instructions.
-   *)
 
   Record validation_exception :=
     mk_ptr_validation_exception
       {
         ptr_expected_zero_offset : bool;
         ptr_deref_beyond_heap_range : bool;
-        ptr_bad_slice: bool;
+        ptr_bad_span: bool;
       }.
 
   Definition no_exceptions : validation_exception
     := mk_ptr_validation_exception false false false.
 
+  Definition heap_ptr_empty := mk_hptr zero32 zero32.
+  Definition span_empty := mk_span zero32 zero32.
+
+  Definition free_ptr_empty :=
+    {|
+      p_span := span_empty;
+      p_offset:= zero32;
+    |}.
+
   Definition fat_ptr_empty :=
     {|
       fp_page := None;
-      fp_start := zero32;
-      fp_length:= zero32;
-      fp_offset:= zero32;
+      fp_ptr := free_ptr_empty;
     |}.
 
-  Definition is_overflowing {bits:nat} (res: int_mod bits* bool) := snd res.
 
-  Definition validate (p:fat_ptr) (fresh:bool) : validation_exception :=
-    {|
-      ptr_expected_zero_offset    := fresh && negb (p.(fp_offset) == zero32);
-      ptr_deref_beyond_heap_range := is_overflowing (p.(fp_start) + p.(fp_length));
-      ptr_bad_slice := gt_unsigned _ p.(fp_offset) p.(fp_length);
-    |}.
+  (** A pointer may be invalid in three cases:
+ 1. A fresh pointer
+ 2. 
+   *)
+  Definition validate (p:free_ptr) (fresh:bool) : validation_exception :=
+    match p with
+      | mk_ptr (mk_span start len) ofs =>
+          {|
+            ptr_expected_zero_offset    := fresh && negb (ofs == zero32);
+            ptr_deref_beyond_heap_range := is_overflowing _ (start + len);
+            ptr_bad_span := ofs > len;
+          |}
+      end.
 
   Definition validate_fresh p := validate p true.
   Definition validate_non_fresh p := validate p false.
 
 
-  Definition is_trivial (p:fat_ptr) := (p.(fp_length) == zero32) && (p.(fp_offset)
-                                                                     == zero32).
+  Definition is_trivial (p:free_ptr) := (p.(s_length) == zero32) && (p.(p_offset) == zero32).
 
-  Inductive fat_ptr_shrink : fat_ptr -> fat_ptr -> Prop :=
-  | fps_shrink : forall p start start' length length' ofs,
-      validate (mk_fat_ptr p start length ofs) false = no_exceptions ->
+  (** Shrinking trims the part of the memory span, defined by a fat pointer, from its start to the offset.
+
+Shrinking happens in two situations:
+
+- far calls with forwarding mode [%ForwardFatPointer];
+- returns from far calls with forwarding mode [%ForwardFatPointer].
+
+   *)
+  Inductive free_ptr_shrink : free_ptr -> free_ptr -> Prop :=
+  | tps_shrink : forall start start' length length' ofs,
+      validate (mk_ptr (mk_span start length) ofs) false = no_exceptions ->
       start + ofs = (start', false) ->
       length - ofs = (length', false) ->
-      fat_ptr_shrink (mk_fat_ptr p start length ofs) (mk_fat_ptr p start' length' zero32).
+      free_ptr_shrink (mk_ptr (mk_span start length) ofs) (mk_ptr (mk_span start' length') zero32).
 
-  (** Used by [OpPtrShrink] instruction. *)
-  Inductive fat_ptr_trim_length : fat_ptr -> mem_address -> fat_ptr -> Prop :=
-  | fptl_apply: forall p start diff length length' ofs,
+  Definition fp_shrink := fp_lift free_ptr_shrink.
+
+  (** Used by [%OpPtrShrink] instruction. *)
+
+  Inductive hptr_trim_length (diff: mem_address) : heap_ptr -> heap_ptr -> Prop :=
+  | tptl_apply: forall length length' ofs,
       length - diff = (length', false) ->
-      fat_ptr_trim_length (mk_fat_ptr p start length ofs) diff (mk_fat_ptr p start length' ofs).
+      hptr_trim_length diff (mk_hptr ofs length) (mk_hptr ofs length').
+
+  Inductive span_trim_length (diff: mem_address) : span -> span -> Prop :=
+  | stl_apply: forall start length length',
+      length - diff = (length', false) ->
+      span_trim_length diff (mk_span start length) (mk_span start length').
 
   Definition growth (current_bound: mem_address) (query_bound: mem_address)
     : mem_address :=
-    if le_unsigned _ query_bound current_bound then zero32 else
-      fst (usub_overflow _ query_bound current_bound).
+    if query_bound < current_bound then zero32 else
+      fst (query_bound - current_bound).
 
-  Inductive fat_ptr_induced_growth: fat_ptr -> forall current_bound: mem_address, mem_address -> Prop :=
-  | gb_bytes: forall fp_page fp_start fp_length fp_offset query_bound current_bound,
+  Inductive span_induced_growth: span -> forall current_bound: mem_address, mem_address -> Prop :=
+  | gb_bytes: forall fp_start fp_length query_bound current_bound,
       fp_start + fp_length = (query_bound, false) ->
       let diff := growth current_bound query_bound in
-      fat_ptr_induced_growth (mk_fat_ptr fp_page fp_start fp_length fp_offset) current_bound diff.
+      span_induced_growth (mk_span fp_start fp_length) current_bound diff.
 
-  Inductive ptr_inc : fat_ptr -> fat_ptr -> Prop :=
+
+  Inductive hptr_inc : heap_ptr -> heap_ptr -> Prop :=
   |fpi_apply :
-    forall page start len ofs ofs',
+    forall ofs ofs' lim,
       ofs + (u32_of z_bytes_in_word) = (ofs', false) ->
-      ptr_inc (mk_fat_ptr page start len ofs) (mk_fat_ptr page start len ofs').
+      hptr_inc (mk_hptr ofs lim) (mk_hptr ofs' lim).
+
+  Inductive ptr_inc : free_ptr -> free_ptr -> Prop :=
+  |fpf_apply :
+    forall ofs ofs' s,
+      ofs + (u32_of z_bytes_in_word) = (ofs', false) ->
+      ptr_inc (mk_ptr s ofs) (mk_ptr s ofs').
 
 
-  (** ### Data slices
+  Definition fp_inc := fp_lift ptr_inc.
+  (** ### Slices
 
+Accesses through fat pointers should be in bounds from [%fp_start] (inclusive) to [%fp_start]+[%fp_length] (exclusive).
 
-Accesses through fat pointers should be in bounds from [fp_start] (inclusive) to [fp_start]+[fp_length] (exclusive).
-
-Accesses through [OpLoadPtr] and [OpLoadPtrInc] return 32-byte words starting at an address [fp_start + fp_offset], specified by  fat pointer.
-However, the word might surpass the upper bound when [fp_length - fp_offset <= 32].
+Accesses through [%OpLoadPtr] and [%OpLoadPtrInc] return 32-byte words starting at an address [%fp_start + fp_offset], specified by  fat pointer.
+However, the word spans across addresses from [%fp_start + fp_offset] to [%fp_start + fp_offset + 32] and might surpass the upper bound when [%fp_length - fp_offset <= 32].
 In this case, reads from out-of-bound bytes will return zero bytes.
 
 
@@ -122,19 +226,25 @@ Data slice is a virtual memory page holding a read-only fragment of some memory 
   Definition data_page_slice_params := data_page_params <| writable := false |>.
   Definition data_slice := mem_parameterized data_page_slice_params.
 
-  Definition slice  (from_incl to_excl: mem_address) (m:data_page) : data_slice :=
+  Definition do_slice_page (from_incl to_excl: mem_address) (m:data_page) : data_slice :=
     let from_key := MemoryBase.addr_to_key _ from_incl in
     let to_key := MemoryBase.addr_to_key _ to_excl in
     let contents := pmap_slice m from_key to_key in
     mk_mem data_page_slice_params contents.
 
 
-  (** Predicate [slice_from_ptr] describes a slice corresponding to a fat pointer pointer. *)
-  Inductive slice_from_ptr (m:data_page) : fat_ptr -> data_slice -> Prop :=
+  (** Predicate [%slice_page] describes a slice visible to a fat pointer. *)
+  Inductive slice_page (m:data_page) : span -> data_slice -> Prop :=
   | sfp_apply:
-    forall page start length ofs upper_bound readonly_slice,
+    forall start length upper_bound readonly_slice,
       start + length = (upper_bound, false) ->
-      slice start upper_bound  m = readonly_slice ->
-      slice_from_ptr m (mk_fat_ptr  page start length ofs) readonly_slice.
+      do_slice_page start upper_bound  m = readonly_slice ->
+      slice_page m (mk_span start length) readonly_slice.
 
 End Definitions.
+
+Module Coercions.
+
+  Coercion heap_ptr_to_free : heap_ptr >-> free_ptr.
+
+End Coercions .
