src/Coder.v
@@ -4,29 +4,29 @@ Section Encoding.
 
 Application Binary Interfaces (ABI) require describing serialization and deserialization.
 
-- Serialization encodes an instance of type [T] into a word of type [word].
-- Deserialization tries to decode an instance of type [T] from a word of type [word].
+- Serialization encodes an instance of type [%T] into a word of type [%word].
+- Deserialization tries to decode an instance of type [%T] from a word of type [%word].
 *)
 
 Context {word T:Type}.
 
-(** Definition [decoder] defines an embedding of a subset of words of type
-[word] to a type [T]. Decoding may fail if the input word is malformed. *)
+(** Definition [%decoder] defines an embedding of a subset of words of type
+[%word] to a type [%T]. Decoding may fail if the input word is malformed. *)
 Definition decoder := word -> option T.
 
-(** Definition [encoder] defines an embedding of type [T] to a set of possible [word] values.
+(** Definition [%encoder] defines an embedding of type [%T] to a set of possible [%word] values.
  Encoding always succeeds. *)
 Definition encoder := T -> word.
 
-(** The record [coder] connects a specific decoder with the matching encoder, and proofs of their properties.
+(** The record [%coder] connects a specific decoder with the matching encoder, and proofs of their properties.
 
-- [revertible1] formalizes the following: if we encode an element [t] of type [T] to a word, and then decode this word, the result will be [t] again.
-- [revertible2] formalizes the following: if we successfully decoded an element [t] of type [T] from a word [w], and then encode [t] again, the encoding will match [w] again. *)
+- [%revertible1] formalizes the following: if we encode an element [%t] of type [%T] to a word, and then decode this word, the result will be [%t] again.
+- [%revertible2] formalizes the following: if we successfully decoded an element [%t] of type [%T] from a word [%w], and then encode [%t] again, the encoding will match [%w] again. *)
 Record coder  := {
     decode: decoder;
     encode:  encoder;
 
-    (** [decode] and [encode] should be mutual inverses. *)
+    (** [%decode] and [%encode] should be mutual inverses. *)
     revertible1: forall params, decode (encode params) = Some params;
     revertible2: forall params encoded, decode encoded = Some params -> encode params = encoded;
   }.
