src/Core.v
@@ -1,24 +1,61 @@
 Require Common lib.ZMod.
 
 Import ZMod Common ZArith.
-(**
-A **word** is a 256-bit unsigned number.
-
-A **cell** is a memory unit for stack, registers, storage  an alias for word.
- *)
-
-Definition word_bits: nat := 256.
+Section Parameters.
+  Open Scope ZMod_scope.
 
 
+  (**
 
-Definition word: Set := ZMod.int_mod word_bits.
-Definition word0: word := ZMod.int_mod_of word_bits 0%Z.
+# EraVM architecture overview
 
-Section Helpers.
+
+EraVM is a 256-bit register-based language machine with stack, dedicated memory for code, data, stack and constants.
+   *)
+  Definition word_bits: nat := 256.
+
+  Definition word: Set := int_mod word_bits.
+  (**
+![](img/arch-overview.png)
+
+
+- **Memory**, provides access to transient memory, consisting of pages. See [%Memory].
+- **Storage**, provides access to persistent storage with two shards, each shard maps $2^{160}$ contracts, to a key-value storage. See [%Memory] and [%Storage].
+- **EventSink**, collects events and L2→L1 messages. See [%Events].
+- **Precompile processor** executes precompiles e.g. `keccak256`, `sha256`, and so on. See [%Precompiles].
+- **Decommittement processor**, stores and decommits the code of contracts. See [%Decommitter].
+
+
+## Execution state
+
+EraVM's functionality is to sequentially execute instructions.
+
+The main components of EraVM's execution state are:
+
+- 256-bit tagged general-purpose registers R1--R15 and a reserved register R0 holding a constant 0. See [%GPR.regs_state].
+- Three flags: overflow/less-than, equals, greater-than. See [%Condition.flags_state].
+- Callstack, holding callframes, which include program counter, stack pointer, current ergs balance, current contract's address, and so on. See [%CallStack].
+- Stack holding tagged words.
+- Read-only pages for constants and code, one per contract stack frame.
+
+First contracts are marked as system, so VM executes them in kernel mode, allowing an access to a richer instruction set. See [%KernelMode].
+
+
+Instructions and some other actions should be paid for with **ergs**, an analogue of gas. See the overview in [%Ergs].
+
+All instructions contain an encoded execution condition. It means that before executing any instruction flags are checked, and if they do not match the required condition, the instruction is skipped.
+
+
+
+   *)
+
+
+  (** [%word0] is a word with a zero value. *)
+  Definition word0: word := int_mod_of word_bits 0%Z.
   Import Nat.
   Definition bytes_in_word : nat := word_bits/bits_in_byte.
   Definition z_bytes_in_word : Z := Z.of_nat bytes_in_word.
-End Helpers.
+End Parameters.
 
 
 Definition timestamp := nat.
