src/Memory.v
@@ -11,21 +11,21 @@ Import ListNotations.
 All memory available to the contract code can be divided into transient and persistent memory.
 
 - Transient memory exists to enable computations and does not persist between VM, like the main memory of personal computers.
-- Persistent memory exists as a storage of untagged 256-bit [word]s shared between the network participants.
+- Persistent memory exists as a storage of untagged 256-bit [%word]s shared between the network participants.
 
 Contract code uses transient memory to perform computations and uses the storage to publish its results
 
 
 ## Persistent memory
 
-The global persistent data structure is the [depot]. It holds untagged 256-bit words.
+The global persistent data structure is the [%depot]. It holds untagged 256-bit words.
 
-Depot is split in two [shard]s: one corresponds to rollup, another to porter (see [shard_exists]).
+Depot is split in two [%shard]s: one corresponds to rollup, another to porter (see [%shard_exists]).
 
-Each shard is a map from a [contract_address] (160 bit, might be extended in
-future to up to 256 bits) to contract [storage].
+Each shard is a map from a [%contract_address] (160 bit, might be extended in
+future to up to 256 bits) to contract [%storage].
 
-Each contract [storage] is a linear mapping from $2^{256}$ **keys** to 256-bit untagged words.
+Each contract [%storage] is a linear mapping from $2^{256}$ **keys** to 256-bit untagged words.
 
 Therefore, the **fully qualified address** of a word in depot is:
 
@@ -35,13 +35,13 @@ $(\texttt{shard\_id}, \texttt{contract\_id} , \texttt{key})$
 
 Contract has one independent storage per shard.
 
-One shard is selected as currently active in [State].
+One shard is selected as currently active in [%State].
 
 Contract code is shared between shards.
 
 ## Transient memory
 
-Transient memory consists of [page]s holding data or code.
+Transient memory consists of [%page]s holding data or code.
 Each page holds $2^{32}$ bytes; all bytes are initialized to zero at genesis.
 
 New pages are allocated implicitly when the contract execution starts; calling another contract allocates more pages.
@@ -86,13 +86,13 @@ Definition storage: Type := mem_parameterized storage_params.
 Definition storage_empty : storage := empty storage_params.
 
 (**
-Storage does not hold contract code, it is a responsibility of decommittment processor [decommitter].
+Storage does not hold contract code, it is a responsibility of decommittment processor [%decommitter].
 
-Storage is a part of a [shard], which is a part of [depot].
+Storage is a part of a [%shard], which is a part of [%depot].
 
 ## Instructions
 
-Instruction [OpSLoad] implements reading from storage; instruction [OpSStore] implements writing to storage.
+Instruction [%OpSLoad] implements reading from storage; instruction [%OpSStore] implements writing to storage.
 
 ## Memory model
 
@@ -102,7 +102,7 @@ All writes are atomic and immediately visible; reads are guaranteed to return th
 
 # Shards and contracts
 
-A **contract** is uniquely identified by its 160-bit address [contract_address].
+A **contract** is uniquely identified by its 160-bit address [%contract_address].
 In future, the address could be seemlessly extended to up to 256 bits.
 
 A **shard** is a mapping of contract addresses to storages.
@@ -122,10 +122,10 @@ Definition contract_address_bits := address_bits shard_params.
 Definition shard := mem_parameterized shard_params.
 
 (** Contracts are also associated with code. The association is global per depot
-and implemented by [Decommitter]. Therefore, the contract code is the same for all
+and implemented by [%Decommitter]. Therefore, the contract code is the same for all
 shards, but the storages of a contract in different shards differ.
 
-Contracts with addresses in range from 0 (inclusive) to [KERNEL_MODE_MAXADDR]
+Contracts with addresses in range from 0 (inclusive) to [%KERNEL_MODE_MAXADDR]
 (exclusive) are **system contracts**; they are allowed to execute all
 instructions.
 
@@ -165,11 +165,11 @@ Contract execution routinely uses **main memory** to hold instructions, stack, h
 
 When the execution of a contract starts, new pages are allocated for:
 
-- contract code: [code_page], fetched by decommitter; see [Decommitter] and [FarCall]);
-- data stack: [stack_page];
-- heap: [data_page];
-- aux_heap: [data_page];
-- constants: [const_page], implementation may chose to allocate code and constants on the same page.
+- contract code: [%code_page], fetched by decommitter; see [%Decommitter] and [%FarCall]);
+- data stack: [%stack_page];
+- heap: [%data_page];
+- aux_heap: [%data_page];
+- constants: [%const_page], implementation may chose to allocate code and constants on the same page.
 
 Therefore, the types of pages are: data pages, stack pages, constant data pages, and code pages. **)
 
@@ -193,7 +193,7 @@ Therefore, the types of pages are: data pages, stack pages, constant data pages,
     | CodePage : code_page -> page.
 
 
-    (** **Memory** is a collection of pages [memory], each page is attributed a unique identifier [page_id]. Pages persist for as long as they can be read by some code; in presence of [FatPointer] the page lifetime may exceed the lifetime of the frame that created it. *)
+    (** **Memory** is a collection of pages [%memory], each page is attributed a unique identifier [%page_id]. Pages persist for as long as they can be read by some code; in presence of [%FatPointer] the page lifetime may exceed the lifetime of the frame that created it. *)
 
     Definition page_id := nat.
     Definition memory := list (page_id * page).
@@ -203,7 +203,7 @@ Therefore, the types of pages are: data pages, stack pages, constant data pages,
         List.In (id, page) mm ->
         page_has_id mm id page.
 
-    (** The set of identifiers has a complete linear order, ordering the pages by the time of creation. The ability to distinguish older pages from newer is necessary to prevent returning fat pointers to pages from older frames. See e.g. [step_retext]. *)
+    (** The set of identifiers has a complete linear order, ordering the pages by the time of creation. The ability to distinguish older pages from newer is necessary to prevent returning fat pointers to pages from older frames. See e.g. [%step_retext]. *)
 
     Section Order.
       Definition page_ordering := Nat.leb.
@@ -213,9 +213,9 @@ Therefore, the types of pages are: data pages, stack pages, constant data pages,
         page_ordering id1 id2.
     End Order.
 
-    (** Predicate [page_replace] describes a relation between two memories [m1]
-    and [m2], where [m2] is a copy of [m1] but a page with it [id] is replaced
-    by another page [p].*)
+    (** Predicate [%page_replace] describes a relation between two memories [%m1]
+    and [%m2], where [%m2] is a copy of [%m1] but a page with it [%id] is replaced
+    by another page [%p].*)
     Inductive page_replace (id:page_id) (p:page): memory -> memory -> Prop :=
     | mm_replace_base: forall oldpage newpage tail,
         page_replace id p ((id, oldpage)::tail) ((id,newpage)::tail)
@@ -224,7 +224,7 @@ Therefore, the types of pages are: data pages, stack pages, constant data pages,
         id <> not_id ->
         page_replace id p ((not_id,oldpage)::tail) ((not_id,oldpage)::tail').
 
-    (** Function [page_alloc] creates a new page in memory. *)
+    (** Function [%page_alloc] creates a new page in memory. *)
     Definition page_alloc (p:page) (m: memory ) : memory :=
       let new_id := length m in
       cons (new_id, p) m.
@@ -250,18 +250,20 @@ A **data page** contains individually addressable bytes. Each data page holds $2
 
   Definition data_page := mem_parameterized data_page_params.
 
-  (** There are currently two types of data pages: [Heap] and [AuxHeap] pages. *)
+  (** There are currently two types of data pages: [%Heap] and [%AuxHeap] pages.
+  We call both of them **heap variants** for brevity, as working with them is
+  quite similar. *)
   Inductive data_page_type := Heap | AuxHeap.
 
 
-(** Note: only instructions from UMA (unaligned memory access) instruction family can access data pages ([OpLoad]/[OpLoadInc], [OpStore]/[OpStoreInc], [OpLoadPointer]/OpLoadPointerInc]).
+(** Note: only instructions from UMA (unaligned memory access) instruction family can access data pages ([%OpLoad]/[%OpLoadInc], [%OpStore]/[%OpStoreInc], [%OpLoadPointer]/OpLoadPointerInc]).
 Every byte on data pages has an address, but the instructions from UMA family read or store 32-byte words.
 
-Fat pointers [fat_ptr] define slices of data pages and allow passing them between contracts.
+Fat pointers [%fat_ptr] define slices of data pages and allow passing them between contracts.
 
 ### Stack pages
 
-A **stack page** contains $2^{16}$ primitive values (see [primitive_value]).
+A **stack page** contains $2^{16}$ primitive values (see [%primitive_value]).
 Therefore, elements of stack pages are tagged words.
 
 *)
@@ -280,7 +282,7 @@ Therefore, elements of stack pages are tagged words.
 
 (** ### Const pages
 
-A **const page** contains $2^{16}$ primitive values (see [primitive_value]).
+A **const page** contains $2^{16}$ primitive values (see [%primitive_value]).
 They are not writable.
 
 Implementation may put constants and code on the same pages.
@@ -304,14 +306,14 @@ They are not writable.
 On genesis, code pages are filled as follows:
 
 - The contract code is places starting from the address 0.
-- The rest is filled with a value guaranteed to decode as invalid instruction [invalid_ins].
+- The rest is filled with a value guaranteed to decode as invalid instruction [%invalid_ins].
 
 Const pages can coincide with code pages.
  *)
 
   Context {ins_type: Type} (invalid_ins: ins_type).
 
-  (* Implementation note: [code_address] should be [address code_page_params] but we don't want to introduce
+  (* Implementation note: [%code_address] should be [%address code_page_params] but we don't want to introduce
       dependency between code_address and instruction type *)
   Definition code_address_bits := 16.
   Definition code_address :=  ZMod.int_mod code_address_bits.
@@ -329,5 +331,5 @@ Const pages can coincide with code pages.
 
 End Memory.
 
-(** The definition [era_pages] collects the specific types of pages used by EraVM semantic. *)
+(** The definition [%era_pages] collects the specific types of pages used by EraVM semantic. *)
 Definition era_pages {instr} {inv:instr} := Build_pages_config (code_page inv) const_page data_page stack_page.
