src/MemoryContext.v
@@ -4,9 +4,17 @@ Require Memory lib.ZMod.
 
 Import List Memory ZMod.
 
-Section Definitions.
+Section MemoryContext.
   Import ListNotations RecordSetNotations.
 
+  Open Scope ZMod_scope.
+
+  (** # Memory context
+
+Creation of a contract frame leads to allocation of pages for code, constant data, stack, and heap variants.
+
+**Memory context** is a collection of these pages associated with a contract frame, plus the bounds for heap variants.
+   *)
   Record mem_ctx :=
     mk_mem_ctx
       {
@@ -19,6 +27,9 @@ Section Definitions.
         ctx_auxheap_bound: mem_address;
       }.
 
+
+  (** The identifiers of pages in [%mem_ctx] are not guaranteed to be in any order. However, we need to be able to tell whether a given page was created before a given memory context; this is formalized by [%page_older].  *)
+
   Definition list_mem_ctx (ap:mem_ctx) : list page_id :=
     match ap with
     | mk_mem_ctx code_id const_id stack_id heap_id auxheap_id _ _ =>
@@ -27,12 +38,20 @@ Section Definitions.
 
   Definition page_older (id: page_id) (mps: mem_ctx) : bool :=
     List.forallb (page_older id) (list_mem_ctx mps).
-  Definition is_active_page (ap:mem_ctx) (id: page_id) : bool :=
-    List.existsb (page_eq id) (list_mem_ctx ap).
 
-  Open Scope ZMod_scope.
+  (** Function [%is_active_page] returns [%true] if memory page [%id] belongs to the context [%c]. *)
+  Definition is_active_page (c:mem_ctx) (id: page_id) : bool :=
+    List.existsb (page_eq id) (list_mem_ctx c).
+
 
   #[export] Instance etaAP: Settable _ := settable! mk_mem_ctx< ctx_code_page_id; ctx_const_page_id; ctx_stack_page_id; ctx_heap_page_id; ctx_auxheap_page_id; ctx_heap_bound; ctx_auxheap_bound >.
+
+
+  (** If an instruction addresses a heap variant outside of its bounds, its
+  bound is adjusted to include the used address. Then the bound has to be
+  adjusted; predicates [%grow_heap_page], [%grow_auxheap_page],
+  [%grow_heap_variant] are relating memory contexts where an appropriate heap
+  variant was grown. *)
 
   Inductive grow_heap_page: mem_address -> mem_ctx -> mem_ctx -> Prop :=
   | gp_heap: forall ap new_bound diff,
@@ -52,4 +71,4 @@ Section Definitions.
       grow_auxheap_page diff ap ap' ->
       grow_heap_variant AuxHeap diff ap ap'.
 
-End Definitions.
+End MemoryContext.
