src/PrimitiveValue.v
@@ -1,9 +1,14 @@
 (**
- **Primitive value** is a tagged word. The tag shows that the word contains a valid fat pointer (see [ABI.FatPointer]) and can be used in instructions that require pointer argument, for example [OpPtrShrink].
+ # Primitive values
 
-Only registers and stack hold primitive values; other types of memory, including storage, holds non-tagged words. *)
+**Primitive value** is a tagged word. The tag shows that the word contains a
+  valid fat pointer (see [%fat_ptr]) and can be used in instructions that
+  require pointer argument, for example [%OpPtrShrink].
 
-Section Definitions.
+Only registers and stack hold primitive values; other types of memory, including storage, holds non-tagged words.
+ *)
+
+Section PrimitiveValue.
 Context {word:Type}.
 Inductive primitive_value :=
   mk_pv {
@@ -11,12 +16,13 @@ Inductive primitive_value :=
       value: word;
     }.
 
-(** Function [clear_pointer_tag] clears the pointer tag of a primitive value. *)
+(** Function [%clear_pointer_tag] clears the pointer tag of a primitive value. *)
 Definition clear_pointer_tag (pv:primitive_value): primitive_value :=
   match pv with | mk_pv _ value => mk_pv false value end.
 
-End Definitions.
+End PrimitiveValue.
 
-
+(** For brevity, we will call a primitive value **a pointer value** if its tag
+is set, and **integer value** otherwise. *)
 Notation IntValue := (mk_pv false).
 Notation PtrValue := (mk_pv true).
