src/sem/Farcall.v
@@ -1,5 +1,5 @@
 From RecordUpdate Require Import RecordSet.
-Require Common Decommitter Ergs Condition CallStack Memory Instruction State MemoryOps ABI SemanticCommon.
+Require Common Decommitter Ergs Condition CallStack Memory Instruction State MemoryOps ABI Pointer SemanticCommon.
 
 Import
   BinIntDef.Z
@@ -41,21 +41,21 @@ Local Coercion int_mod_of : Z >-> int_mod.
 Far calls are calls to the code outside the current contract space.
 This file describes three instructions to perform far calls:
 
-- [OpFarCall]
-- [OpDelegateCall]
-- [OpMimicCall] (available only in kernel mode)
+- [%OpFarCall]
+- [%OpDelegateCall]
+- [%OpMimicCall] (available only in kernel mode)
 
 These instructions differ in the way they construct new frame.
 
 The far call instructions have rich semantics; their full effect on the
 VM state is described through the following main predicates:
 
-- [Semantics.step]
-- [step]
-- [fetch_operands]
-- [farcall]
+- [%Semantics.step]
+- [%step]
+- [%fetch_operands]
+- [%farcall]
 
-If you know about fetching operands for instructions and the instruction fetching described in [Semantics.step], start investigating farcalls from the [farcall] predicate.
+If you know about fetching operands for instructions and the instruction fetching described in [%Semantics.step], start investigating farcalls from the [%farcall] predicate.
  *)
 Section Parameters.
   Open Scope Z_scope.
@@ -68,10 +68,10 @@ Section Parameters.
 1. Initial preallocated stack space.
 
    A far call creates a new context with a new stack page (and other pages, see
-   [page_alloc]).
-   The initial SP value after a far call is set to [INITIAL_SP_ON_FAR_CALL].
+   [%page_alloc]).
+   The initial SP value after a far call is set to [%INITIAL_SP_ON_FAR_CALL].
 
-   Therefore, addresses in range from 0 inclusive to [INITIAL_SP_ON_FAR_CALL]
+   Therefore, addresses in range from 0 inclusive to [%INITIAL_SP_ON_FAR_CALL]
    exclusive can be used as a scratch space.
    *)
 
@@ -80,7 +80,7 @@ Section Parameters.
   (**
 2. Initial heap and auxheap pages bound.
 
-   The heap and auxheap pages start with [NEW_FRAME_MEMORY_STIPEND] bound.
+   The heap and auxheap pages start with [%NEW_FRAME_MEMORY_STIPEND] bound.
    Growing them beyond this bound costs ergs.
    *)
   Definition NEW_FRAME_MEMORY_STIPEND : mem_address := 1024.
@@ -94,15 +94,15 @@ End Parameters.
  *)
 Definition max_passable (remaining:ergs) : ergs := (((int_val _ remaining) / 64 ) * 63)%Z.
 Inductive pass_allowed_ergs : (ergs * callstack )-> ergs * callstack -> Prop :=
-| pae_apply: forall xstack1 xstack2 pass_ergs_query,
-    let pass_ergs_actual := ZMod.min _ (max_passable (ergs_remaining xstack1)) pass_ergs_query in
-    pay pass_ergs_actual xstack1 xstack2 ->
+| pae_apply: forall cs1 cs2 pass_ergs_query,
+    let pass_ergs_actual := ZMod.min _ (max_passable (ergs_remaining cs1)) pass_ergs_query in
+    pay pass_ergs_actual cs1 cs2 ->
     pass_ergs_query <> zero32 ->
-    pass_allowed_ergs (pass_ergs_query,xstack1) (pass_ergs_actual, xstack2)
-| pae_zero: forall xstack1 xstack2,
-    let pass_ergs_actual := max_passable (ergs_remaining xstack1) in
-    pay pass_ergs_actual xstack1 xstack2 ->
-    pass_allowed_ergs (zero32, xstack1) (pass_ergs_actual, xstack2).
+    pass_allowed_ergs (pass_ergs_query,cs1) (pass_ergs_actual, cs2)
+| pae_zero: forall cs1 cs2,
+    let pass_ergs_actual := max_passable (ergs_remaining cs1) in
+    pay pass_ergs_actual cs1 cs2 ->
+    pass_allowed_ergs (zero32, cs1) (pass_ergs_actual, cs2).
 
 
 (**
@@ -117,7 +117,7 @@ Far call creates a new execution context with new pages for:
 - heap
 - auxheap
 
-The initial bounds for the new heap and auxheap pages are set to [NEW_FRAME_MEMORY_STIPEND].
+The initial bounds for the new heap and auxheap pages are set to [%NEW_FRAME_MEMORY_STIPEND].
  *)
 Inductive alloc_pages_extframe:  (memory * mem_ctx) -> code_page -> memory * mem_ctx -> Prop :=
 | ape_alloc: forall code mm ctx code_id const_id stack_id heap_id heap_aux_id,
@@ -149,33 +149,33 @@ Otherwise, it costs the amount of ergs proportionate to the code size (in words)
  *)
 Inductive decommitment_cost (cm:decommitter) vhash (code_length_in_words: code_length): ergs -> Prop :=
 |dc_fresh: forall cost,
-    is_fresh _ cm vhash = true->
+    is_first_access _ cm vhash = true->
     (cost, false) = umul_overflow _ Ergs.ERGS_PER_CODE_WORD_DECOMMITTMENT (resize _ _ code_length_in_words) ->
     decommitment_cost cm vhash code_length_in_words cost
 |dc_not_fresh:
-  is_fresh _  cm vhash = false ->
+  is_first_access _  cm vhash = false ->
   decommitment_cost cm vhash code_length_in_words zero32.
 
-(** Fetch code and pay the associated cost. If [masking_allowed] is true and there is no code
+(** Fetch code and pay the associated cost. If [%masking_allowed] is true and there is no code
 associated with a given contract address, then the default AA code will be
-fetched. See [code_fetch]. *)
+fetched. See [%code_fetch]. *)
 Inductive paid_code_fetch masking_allowed sid: depot -> decommitter -> contract_address
                                            -> callstack -> callstack * code_page
                                            ->Prop :=
 | cfp_apply:
-  forall depot (codes:decommitter) (dest_addr: contract_address) vhash dest_addr new_code_page code_length cost__decomm xstack0 xstack1,
+  forall depot (codes:decommitter) (dest_addr: contract_address) vhash dest_addr new_code_page code_length cost__decomm cs0 cs1,
 
     code_fetch _ depot codes.(cm_storage _) sid dest_addr masking_allowed (vhash, new_code_page, code_length) ->
     decommitment_cost codes vhash code_length cost__decomm ->
-    pay cost__decomm xstack0 xstack1 ->
-    paid_code_fetch masking_allowed sid depot codes dest_addr xstack0 (xstack1, new_code_page).
+    pay cost__decomm cs0 cs1 ->
+    paid_code_fetch masking_allowed sid depot codes dest_addr cs0 (cs1, new_code_page).
 
 (** ## System calls
 
 A system call is a far call that satisfies the following conditions:
 
 - The destination is a kernel address.
-- The field `is_system` of [FarCall.params] passed through an operand is set to 1.
+- The field `is_system` of [%FarCall.params] passed through an operand is set to 1.
  *)
 
 
@@ -187,7 +187,7 @@ A system call is a far call that satisfies the following conditions:
 
 - Mimic calls are a kernel-only variation of far calls allowing to mimic a call
   from any contract by impersonating an arbitrary caller and putting an arbitrary
-  address into the new callframe's [ecf_msg_sender] field.
+  address into the new callframe's [%ecf_msg_sender] field.
 
 - Delegate calls are a variation of far calls allowing to call a contract with the current storage space.
 
@@ -200,7 +200,7 @@ A system call is a far call that satisfies the following conditions:
 
 ## Syntax
 
-- [OpFarCall] `abi_params address handler is_static`
+- [%OpFarCall] `abi_params address handler is_static`
    + `farcall        abi_reg, dest_addr`
    + `farcall        abi_reg, dest_addr, handler `
    + `farcall.static abi_reg, dest_addr`
@@ -208,7 +208,7 @@ A system call is a far call that satisfies the following conditions:
    + `farcall.shard  abi_reg, dest_addr`
    + `farcall.shard  abi_reg, dest_addr, handler`
 
-- [OpDelegateCall] abi_params address handler is_static`
+- [%OpDelegateCall] abi_params address handler is_static`
    + `delegatecall        abi_reg, dest_addr`
    + `delegatecall        abi_reg, dest_addr, handler`
    + `delegatecall.static abi_reg, dest_addr`
@@ -216,7 +216,7 @@ A system call is a far call that satisfies the following conditions:
    + `delegatecall.shard  abi_reg, dest_addr`
    + `delegatecall.shard  abi_reg, dest_addr, handler`
 
-- [OpMimicCall] `abi_params address handler is_static`
+- [%OpMimicCall] `abi_params address handler is_static`
    + `mimic        abi_reg, dest_addr`
    + `mimic        abi_reg, dest_addr, handler`
    + `mimic.static abi_reg, dest_addr`
@@ -233,12 +233,12 @@ A system call is a far call that satisfies the following conditions:
 ## Semantic
 
 The semantics of all three
-First two steps are formalized by predicates [Semantics.step] and [fetch_operands].
+First two steps are formalized by predicates [%Semantics.step] and [%fetch_operands].
 
 1. Fetch the instruction, adjust PC and perform the usual checks (such as kernel
    mode), pay basic costs, and so on.
 
-   See [Semantics.step] for details.
+   See [%Semantics.step] for details.
 
 2. Retrieve the operands and decode the following structure from `abi_reg`:
 
@@ -253,15 +253,15 @@ First two steps are formalized by predicates [Semantics.step] and [fetch_operand
      }.
 ```
 
-   See [fetch_operands] for details.
+   See [%fetch_operands] for details.
 
-   The [farcall] predicate encodes the important part of instruction semantics for
-   [OpFarCall], [OpDelegateCall], and [OpMimicCall].
+   The [%farcall] predicate encodes the important part of instruction semantics for
+   [%OpFarCall], [%OpDelegateCall], and [%OpMimicCall].
 
-3. Decommit code of the callee contract (formalized by [paid_code_fetch]):
+3. Decommit code of the callee contract (formalized by [%paid_code_fetch]):
 
-   - load the [versioned_hash] of the called code from the storage of a
-     special contract located at [DEPLOYER_SYSTEM_CONTRACT_ADDRESS].
+   - load the [%versioned_hash] of the called code from the storage of a
+     special contract located at [%DEPLOYER_SYSTEM_CONTRACT_ADDRESS].
 
 ```
 Inductive marker := CODE_AT_REST | YET_CONSTRUCTED | INVALID.
@@ -273,28 +273,28 @@ Record versioned_hash := {
 }.
 ```
    - for non-system calls, if there is no code stored for a provided hash value,
-     mask it into [VersionedHash.DEFAULT_AA_VHASH] and execute
-     [VersionedHash.DEFAULT_AA_CODE].
+     mask it into [%VersionedHash.DEFAULT_AA_VHASH] and execute
+     [%VersionedHash.DEFAULT_AA_CODE].
 
    - if the code with such hash has not been accessed in the current block, pay
      for decommitment.
 
-4. Forward data to the new frame (formalized by [paid_forward_and_adjust_bounds]).
+4. Forward data to the new frame (formalized by [%paid_forward_and_adjust_bounds]).
 
-   - use the forwarding mode from `abi_reg` -> [forwarding_mode]. Can be `ForwardFatPointer`, `UseHeap` or `UseAuxHeap`;
-   - take the fat pointer to the data slice is taken from `abi_reg` -> [memory_quasi_fat_ptr];
+   - use the forwarding mode from `abi_reg` -> [%forwarding_mode]. Can be `ForwardFatPointer`, `UseHeap` or `UseAuxHeap`;
+   - take the fat pointer to the data slice is taken from `abi_reg` -> [%memory_quasi_fat_ptr];
    - for the forwarding mode `ForwardFatPointer`:
      - check the pointer validity;
      - shrink the pointer;
      - ensure that `abi_reg` is tagged as a pointer.
    - for the forwarding modes `UseHeap`/`UseAuxHeap`:
      - check the pointer validity;
-     - overwrite the pointer's [page_id] with the ID of current (aux)heap's memory page;
+     - overwrite the pointer's [%page_id] with the ID of current (aux)heap's memory page;
      - if the pointer bounds surpass current heap/auxheap bounds, pay for growth
        and adjust the bounds of heap/auxheap in the current stack frame.
 
-5. Allocate new pages for code, constants, stack, heap and auxheap (formalized by [alloc_pages_extframe]).
-6. Reserve ergs for the new external frame (formalized by [pass_allowed_ergs]).
+5. Allocate new pages for code, constants, stack, heap and auxheap (formalized by [%alloc_pages_extframe]).
+6. Reserve ergs for the new external frame (formalized by [%pass_allowed_ergs]).
 
    - Maximum amount of ergs passed to an external call is 63/64 of current balance.
    - Attempting to pass more ergs will result in only passing the maximum amount allowed.
@@ -302,16 +302,16 @@ Record versioned_hash := {
 
 7. Clear the context register.
 8. Clear flags.
-9. Modify GPRs depending on the call being system or not (formalized by [regs_effect]):
+9. Modify GPRs depending on the call being system or not (formalized by [%regs_effect]):
 
   - Effect of a non-system call:
     + All registers are cleared.
     + Register `R1` is assigned a fat pointer to forward data to the far call.
-      See [paid_forward].
+      See [%paid_forward].
 
   - Effect of a system call:
     + Register `R1` is assigned a fat pointer to forward data to the far call.
-      See [paid_forward].
+      See [%paid_forward].
     + Register `R2` is assigned a bit-value:
       - bit 1 indicates "this is a system call"
       - bit 0 indicates "this is a constructor call"
@@ -354,7 +354,7 @@ Definition regs_effect regs (is_system is_ctor:bool) ptr :=
    - set exception handler to `handler` address provided in the instruction;
    - it is a checkpoint that saves all storage states;
    - start PC at 0;
-   - start SP at [INITIAL_SP_ON_FAR_CALL];
+   - start SP at [%INITIAL_SP_ON_FAR_CALL];
  *)
 
 Definition CALL_IMPLICIT_PARAMETER_REG := R3.
@@ -362,21 +362,21 @@ Inductive farcall_type : Set := Normal | Mimic | Delegate.
 
 (**
 
-   - `this_address`,`msg_sender` and `context` fields are affected by the [farcall_type] as follows:
+   - `this_address`,`msg_sender` and `context` fields are affected by the [%farcall_type] as follows:
       + Normal far call sets:
         * `this_address` <- destination address;
         * `msg_sender` <- caller address;
-        * `context` <- value of context register [gs_context_u128].
+        * `context` <- value of context register [%gs_context_u128].
 
       + Delegate call sets:
-        * `this_address` <- [this_address] of the current frame;
-        * `msg_sender` <- [msg_sender] of the current frame;
-        * `context` <- [context_u128] of the current frame.
+        * `this_address` <- [%this_address] of the current frame;
+        * `msg_sender` <- [%msg_sender] of the current frame;
+        * `context` <- [%context_u128] of the current frame.
 
       + Mimic call sets:
         * `this_address` <- destination address;
         * `msg_sender` <- value of `r3`;
-        * `context` <- value of context register [gs_context_u128].
+        * `context` <- value of context register [%gs_context_u128].
 
  *)
 Definition select_this_address type (caller dest: contract_address) :=
@@ -420,26 +420,30 @@ Definition select_shards (type: farcall_type) (is_call_shard: bool) (provided: s
 
 Section Def.
 
+  Import Pointer.
   Context (type:farcall_type) (dest_addr:contract_address) (handler_addr: code_address)
     (call_as_static: bool) (to_abi_shard: bool) (abi_ptr_tag: bool).
 
-  Context (xstack0: callstack)
-    (old_extframe := active_extframe xstack0)
+  Context (cs0: callstack)
+    (old_extframe := active_extframe cs0)
     (mem_ctx0 := old_extframe.(ecf_mem_ctx))
     (current_contract := old_extframe.(ecf_this_address))
   .
 
   Inductive farcall : FarCall.params -> state -> state -> Prop :=
-  | farcall_fwd_fatptr: forall flags old_regs old_pages xstack0 xstack1 xstack2 new_caller_stack gs reg_context_u128 new_pages new_code_page new_mem_ctx in_ptr abi_shard ergs_query ergs_actual fwd_mode is_syscall_query out_ptr,
+  | farcall_fwd_fatptr: forall flags old_regs old_pages cs0 cs1 new_caller_stack gs reg_context_u128 new_pages new_code_page new_mem_ctx (in_ptr out_ptr: fat_ptr) abi_shard ergs_query ergs_actual is_syscall_query out_ptr,
       let is_system := addr_is_kernel dest_addr && is_syscall_query in
       let allow_masking := negb is_system in
       let callee_shard := if to_abi_shard then abi_shard else old_extframe.(ecf_shards).(shard_this) in
       abi_ptr_tag = true ->
 
-      paid_code_fetch allow_masking callee_shard gs.(gs_revertable).(gs_depot) gs.(gs_contracts) dest_addr xstack0 (xstack1, new_code_page) ->
-      paid_forward Ret.ForwardFatPointer (in_ptr, xstack1) (out_ptr, xstack2) ->
+      paid_code_fetch allow_masking callee_shard gs.(gs_revertable).(gs_depot) gs.(gs_contracts) dest_addr cs0 (cs1, new_code_page) ->
+
+      validate_non_fresh in_ptr = no_exceptions ->
+      (fp_lift free_ptr_shrink) in_ptr out_ptr ->
+
       alloc_pages_extframe (old_pages,mem_ctx0) new_code_page (new_pages, new_mem_ctx) ->
-      pass_allowed_ergs (ergs_query,xstack2) (ergs_actual, new_caller_stack) ->
+      pass_allowed_ergs (ergs_query,cs1) (ergs_actual, new_caller_stack) ->
 
       let new_stack := ExternalCall {|
                            ecf_this_address := select_this_address type current_contract dest_addr;
@@ -461,10 +465,9 @@ Section Def.
 
       farcall
         {|
-          memory_quasi_fat_ptr := in_ptr;
+          fwd_memory           := ForwardFatPointer out_ptr;
           ergs_passed          := ergs_query;
           FarCall.shard_id     := abi_shard;
-          forwarding_mode      := fwd_mode;
           constructor_call     := false;
           to_system            := is_syscall_query;
         |}
@@ -473,7 +476,7 @@ Section Def.
                         gs_flags        := flags;
                         gs_regs         := old_regs;
                         gs_pages        := old_pages;
-                        gs_callstack    := xstack0;
+                        gs_callstack    := cs0;
                       |};
           gs_context_u128 := reg_context_u128;
 
@@ -491,17 +494,19 @@ Section Def.
 
           gs_global       := gs;
         |}
-  | farcall_fwd_memory: forall gs flags old_regs old_pages xstack0 xstack1 xstack2 new_caller_stack reg_context_u128 new_pages new_code_page new_mem_ctx in_ptr abi_shard ergs_query ergs_actual is_syscall_query out_ptr page_type,
+  | farcall_fwd_memory: forall gs flags old_regs old_pages cs0 cs1 cs2 new_caller_stack reg_context_u128 new_pages new_code_page new_mem_ctx (in_span: span) abi_shard ergs_query ergs_actual is_syscall_query out_ptr page_type,
       let is_system := addr_is_kernel dest_addr && is_syscall_query in
       let allow_masking := negb is_system in
       let callee_shard := if to_abi_shard then abi_shard else old_extframe.(ecf_shards).(shard_this) in
 
-      paid_code_fetch allow_masking callee_shard gs.(gs_revertable).(gs_depot) gs.(gs_contracts) dest_addr xstack0 (xstack1, new_code_page) ->
-      paid_forward (Ret.UseMemory page_type) (in_ptr, xstack1) (out_ptr, xstack2) ->
+      paid_code_fetch allow_masking callee_shard
+        gs.(gs_revertable).(gs_depot) gs.(gs_contracts)
+                                  dest_addr cs0 (cs1, new_code_page) ->
+      paid_forward_heap_span page_type (in_span, cs1) (out_ptr, cs2) ->
 
-      let mem_ctx1 := (active_extframe xstack2).(ecf_mem_ctx) in
+      let mem_ctx1 := (active_extframe cs2).(ecf_mem_ctx) in
       alloc_pages_extframe (old_pages, mem_ctx1) new_code_page (new_pages, new_mem_ctx) ->
-      pass_allowed_ergs (ergs_query,xstack2) (ergs_actual, new_caller_stack) ->
+      pass_allowed_ergs (ergs_query,cs2) (ergs_actual, new_caller_stack) ->
 
       let new_stack := ExternalCall {|
                            ecf_this_address := select_this_address type current_contract dest_addr;
@@ -523,10 +528,9 @@ Section Def.
 
       farcall
         {|
-          memory_quasi_fat_ptr := in_ptr;
+          fwd_memory           := ForwardNewHeapPointer page_type out_ptr;
           ergs_passed          := ergs_query;
           FarCall.shard_id     := abi_shard;
-          forwarding_mode      := Ret.UseMemory page_type;
           constructor_call     := false;
           to_system            := is_syscall_query;
         |}
@@ -535,7 +539,7 @@ Section Def.
                         gs_flags        := flags;
                         gs_regs         := old_regs;
                         gs_pages        := old_pages;
-                        gs_callstack    := xstack0;
+                        gs_callstack    := cs0;
                       |};
           gs_context_u128 := reg_context_u128;
 
@@ -599,19 +603,19 @@ Inductive step : instruction -> smallstep :=
 ## Affected parts of VM state
 
 - flags are cleared
-- registers are affected as described by [regs_effect].
-- new pages appear as described by [alloc_pages_extframe].
+- registers are affected as described by [%regs_effect].
+- new pages appear as described by [%alloc_pages_extframe].
 - context register is zeroed.
-- execution stack is affected in a non-trivial way (see step 10 in description for [farcall]).
+- execution stack is affected in a non-trivial way (see step 10 in description for [%farcall]).
 
 ## Comparison with near calls
 
-- Far calls can not accept more than [max_passable] ergs, while near calls may accept all available ergs.
-- Abnormal returns from far calls through [OpPanic] or [OpRevert] roll back all
+- Far calls can not accept more than [%max_passable] ergs, while near calls may accept all available ergs.
+- Abnormal returns from far calls through [%OpPanic] or [%OpRevert] roll back all
 storage changes that occured during the contract execution.
 
 This includes exceptional situations when an error occured and the current
-instruction is masked as [OpPanic].
+instruction is masked as [%OpPanic].
 
 
 ## Usage
@@ -621,7 +625,7 @@ instruction is masked as [OpPanic].
 
 ## Encoding
 
-- In the encoding, [OpDelegateCall], [OpFarCall], and [OpMimicCall] share the same opcode.
+- In the encoding, [%OpDelegateCall], [%OpFarCall], and [%OpMimicCall] share the same opcode.
 
 
 # Possible exceptions
