src/sem/LoadPtr.v
@@ -71,14 +71,14 @@ fp_offset := 2
 
       load_reg regs arg_enc_ptr (PtrValue enc_ptr) ->
 
-      ABI.(decode) enc_ptr = Some in_ptr ->
+      decode_fat_ptr enc_ptr = Some in_ptr ->
 
       validate_in_bounds in_ptr = true ->
       Some page_id  =in_ptr.(fp_page) ->
       page_has_id mem page_id (@DataPage era_pages selected_page) ->
-      slice_from_ptr selected_page in_ptr slice ->
+      slice_page selected_page in_ptr slice ->
 
-      (addr, false) = in_ptr.(fp_start) + in_ptr.(fp_offset) ->
+      ptr_resolves_to in_ptr addr  ->
       mb_load_slice_result BigEndian slice addr result ->
 
       store_reg regs arg_dest (IntValue result) new_regs ->
