src/sem/PtrAdd.v
@@ -7,6 +7,7 @@ Import Addressing Common CallStack Memory Instruction State ZMod
 
 Section Def.
   Open Scope ZMod_scope.
+  Import Pointer.Coercions.
 (**
 
 # PtrAdd
@@ -41,41 +42,43 @@ $$result := \mathit{op_1}\{255\dots128\} || \texttt{encode}(\mathit{ptr_{out}})$
  *)
 Inductive step : instruction -> xsmallstep :=
 | step_PtrAdd:
-  forall (in1:in_any) (in2:in_reg) (out:out_any) op1 new_ofs op2 swap result ptr_in regs mem cs new_regs new_mem new_cs flags,
+  forall (in1:in_any) (in2:in_reg) (out:out_any) op1 op2 swap result regs mem cs new_regs new_mem new_cs flags ofs new_ofs limit,
 
-    fetch_apply21_swap swap (regs, mem, cs)
+      fetch_apply21_swap swap (regs, mem, cs)
 
-      (in1,PtrValue op1)
-      (InReg in2, IntValue op2)
-      (out,PtrValue result)
+        (      in1, PtrValue op1)
+        (InReg in2, IntValue op2)
+        (      out, PtrValue result)
 
-      (new_regs, new_mem, new_cs) ->
+        (new_regs, new_mem, new_cs) ->
 
-    FatPointer.ABI.(decode) op1 = Some ptr_in   ->
-    let diff := resize _ 32 op2 in
-    (new_ofs, false) = ptr_in.(fp_offset) + diff ->
+      decode_heap_ptr op1 = Some (mk_hptr ofs limit) ->
+      let diff := resize _ 32 op2 in
+      (new_ofs, false) = ofs + diff ->
 
-    let ptr := FatPointer.ABI.(encode) (ptr_in <| fp_offset := new_ofs |>) in
-    let low := resize _ 128 ptr in
-    mix_lower 128 op1 low = result ->
+      let ptr := encode_fat_ptr (mk_fat_ptr None (mk_hptr new_ofs limit)) in
+      let low := resize _ 128 ptr in
 
-    step (OpPtrAdd in1 in2 out swap)
-         {|
-           gs_callstack    := cs;
-           gs_regs         := regs;
-           gs_pages        := mem;
+      result = mix_lower 128 op1 low ->
 
 
-           gs_flags        := flags;
-         |}
-         {|
-           gs_callstack    := new_cs;
-           gs_regs         := new_regs;
-           gs_pages        := new_mem;
+      step (OpPtrAdd in1 in2 out swap)
+           {|
+             gs_callstack    := cs;
+             gs_regs         := regs;
+             gs_pages        := mem;
 
 
-           gs_flags        := flags;
-         |}
+             gs_flags        := flags;
+           |}
+           {|
+             gs_callstack    := new_cs;
+             gs_regs         := new_regs;
+             gs_pages        := new_mem;
+
+
+             gs_flags        := flags;
+           |}
 .
 (** ## Affected parts of VM state
 
